src/rocq/Handlers/MemoryModules/IPtr.v
@@ -1,0 +1,11 @@
+From Vellvm Require Import
+  Numeric.Rocqlib
+  Utilities.
+
+From Vellvm.Semantics Require Import
+  Params.Address
+  Memory.FiniteProvenance
+  VellvmIntegers.
+
+From QuickChick Require Import Show.
+
