src/rocq/Semantics/Params/Address.v
@@ -1,0 +1,38 @@
+(* -------------------------------------------------------------------------- *
+ *                     Vellvm - the Verified LLVM project                     *
+ *                                                                            *
+ *     Copyright (c) 2017 Steve Zdancewic <stevez@cis.upenn.edu>              *
+ *                                                                            *
+ *   This file is distributed under the terms of the GNU General Public       *
+ *   License as published by the Free Software Foundation, either version     *
+ *   3 of the License, or (at your option) any later version.                 *
+ ---------------------------------------------------------------------------- *)
+
+(* begin hide *)
+From Stdlib Require Import OrderedType OrderedTypeEx.
+
+From Vellvm Require Import
+  Utilities
+  Params.Provenance.
+(* end hide *)
+
+(** * Signature for addresses
+    The semantics is functorized by the notion of addresses manipulated by the
+    memory model. This allows us to easily plug different memory models.
+    This module is concretely implemented currently in [Handlers/Memory.v].
+ *)
+Module Type ADDRESS (P : PROVENANCE).
+  Parameter addr : Set.
+  Parameter null : addr.
+
+  (* Coq's logical equality on the pointer data type *)
+  Parameter eq_dec : forall (a b : addr), {a = b} + {a <> b}.
+  (* Parameter different_addrs : forall (a : addr), exists (b : addr), a <> b. *)
+
+  (* Access the provenance for an address *)
+  Parameter address_provenance : addr -> P.Prov.
+
+  (* Debug *)
+  Parameter show_addr : addr -> string.
+End ADDRESS.
+
