src/rocq/Semantics/Params/IPtr.v
@@ -1,0 +1,70 @@
+(* -------------------------------------------------------------------------- *
+ *                     Vellvm - the Verified LLVM project                     *
+ *                                                                            *
+ *     Copyright (c) 2017 Steve Zdancewic <stevez@cis.upenn.edu>              *
+ *                                                                            *
+ *   This file is distributed under the terms of the GNU General Public       *
+ *   License as published by the Free Software Foundation, either version     *
+ *   3 of the License, or (at your option) any later version.                 *
+ ---------------------------------------------------------------------------- *)
+
+(* begin hide *)
+From Vellvm Require Import
+  Utilities
+  Syntax.DynamicTypes
+  Semantics.VellvmIntegers.
+(* end hide *)
+
+Module Type IPTR.
+  Parameter intptr : Type.
+  Parameter zero : intptr.
+
+  Parameter VMemInt_intptr : VMemInt intptr.
+
+  Parameter eq_dec : forall (a b : intptr), {a = b} + {a <> b}.
+  Parameter eqb : forall (a b : intptr), bool.
+
+  Parameter to_Z : forall (a : intptr), Z.
+  Parameter to_unsigned : forall (a : intptr), Z.
+  Parameter from_Z : Z -> EOB intptr.
+
+  Parameter show_intptr : intptr -> string.
+  
+  Parameter from_Z_to_Z :
+    forall (z : Z) (i : intptr),
+      from_Z z = ret i ->
+      to_Z i = z.
+
+  Parameter from_Z_injective :
+    forall (z1 z2 : Z) (i : intptr),
+      from_Z z1 = ret i ->
+      from_Z z2 = ret i ->
+      z1 = z2.
+
+  Parameter to_Z_from_Z :
+    forall (i : intptr),
+      from_Z (to_Z i) = ret i.
+
+  Parameter from_Z_0 :
+    from_Z 0 = ret zero.
+
+  Parameter to_Z_0 :
+    to_Z zero = 0%Z.
+
+  Parameter to_Z_inj :
+    forall x y,
+      to_Z x = to_Z y ->
+      x = y.
+
+  Parameter VMemInt_intptr_dtyp :
+    @mdtyp_of_int intptr VMemInt_intptr = DTYPE_IPTR.
+
+  Parameter VMemInt_intptr_mrepr_from_Z :
+    forall x,
+      @mrepr intptr VMemInt_intptr x = from_Z x.
+
+  Parameter to_Z_to_unsigned :
+    forall x,
+      to_Z x = to_unsigned x.
+End IPTR.
+
