src/rocq/Semantics/Params/Provenance.v
@@ -1,0 +1,150 @@
+(* begin hide *)
+From Stdlib Require Import OrderedType OrderedTypeEx.
+
+From Vellvm Require Import
+  Utilities
+  Syntax.
+(* end hide *)
+
+(* TODO: Should provenance just be a typeclass? *)
+(* Monad class *)
+Class MonadProvenance (Provenance : Type) (M : Type -> Type) : Type :=
+  { fresh_provenance : M Provenance;
+  }.
+
+(* TODO: move this?
+   TODO: Have I crammed too much into this?
+ *)
+Module Type PROVENANCE.
+  (* Types *)
+  (* Morally:
+
+     - Provenance is the base identifier for provenances.
+     - AllocationId is the provenance associated with bytes /
+       locations in memory
+       + This could additionally allow for wildcard provenance for
+         memory locations, for instance.
+     - Prov is the provenance for a pointer.
+       + May have wildcard provenance, or a set of provenances (e.g.,
+         this pointer may be allowed to access several different blocks
+         of memory, but not all).
+  *)
+  Parameter Provenance : Set.
+  Parameter AllocationId : Set.
+  Parameter Prov : Set.
+
+  Parameter wildcard_prov : Prov.
+  Parameter nil_prov : Prov.
+
+  (* Does the provenance set pr allow for access to aid? *)
+  Parameter access_allowed : Prov -> AllocationId -> bool.
+
+  (* Does the first AllocationId have access to the second? *)
+  Parameter aid_access_allowed : AllocationId -> AllocationId -> bool.
+
+  (* Conversions *)
+  Parameter allocation_id_to_prov : AllocationId -> Prov.
+  Parameter provenance_to_allocation_id : Provenance -> AllocationId.
+  Parameter provenance_to_prov : Provenance -> Prov.
+
+  (* Provenance allocation *)
+  Parameter initial_provenance : Provenance.
+  Parameter next_provenance : Provenance -> Provenance.
+
+  Parameter eq_dec :
+    forall (pr pr' : Provenance),
+      {pr = pr'} + {pr <> pr'}.
+
+
+  (* (* Way easier to keep track of provenances in use if they're ordered... *) *)
+  (* Parameter provenance_lt : Provenance -> Provenance -> Prop. *)
+
+  (* (* Lemmas *) *)
+  (* Parameter aid_access_allowed_refl : *)
+  (*   forall aid, aid_access_allowed aid aid = true. *)
+
+  (* Parameter access_allowed_refl : *)
+  (*   forall aid, *)
+  (*     access_allowed (allocation_id_to_prov aid) aid = true. *)
+
+  (* Parameter allocation_id_to_prov_inv: *)
+  (*   forall aid aid', *)
+  (*     allocation_id_to_prov aid = allocation_id_to_prov aid' -> *)
+  (*     aid = aid'. *)
+
+  (* Parameter provenance_to_allocation_id_inv : *)
+  (*   forall pr pr', *)
+  (*     provenance_to_allocation_id pr = provenance_to_allocation_id pr' -> *)
+  (*     pr = pr'. *)
+
+  (* Parameter allocation_id_to_prov_provenance_to_allocation_id : *)
+  (*   forall pr, *)
+  (*     allocation_id_to_prov (provenance_to_allocation_id pr) = provenance_to_prov pr. *)
+
+  (* Parameter provenance_eq_dec_refl : *)
+  (*   forall (pr : Provenance), *)
+  (*     true = (provenance_eq_dec pr pr). *)
+
+  (* Parameter aid_eq_dec : *)
+  (*   forall (aid aid' : AllocationId), *)
+  (*     {aid = aid'} + {aid <> aid'}. *)
+
+  (* Parameter aid_eq_dec_refl : *)
+  (*   forall (aid : AllocationId), *)
+  (*     true = (aid_eq_dec aid aid). *)
+
+  (* Parameter access_allowed_Proper : *)
+  (*   Proper (eq ==> (fun aid aid' => true = (aid_eq_dec aid aid')) ==> eq) access_allowed. *)
+
+  (* Parameter provenance_lt_trans : Transitive provenance_lt. *)
+
+  (* Parameter provenance_lt_next_provenance : *)
+  (*   forall pr, *)
+  (*     provenance_lt pr (next_provenance pr). *)
+
+  (* Parameter provenance_lt_nrefl : *)
+  (*   forall pr, *)
+  (*     ~ provenance_lt pr pr. *)
+
+  (* Parameter provenance_lt_antisym : Antisymmetric Provenance eq provenance_lt. *)
+
+  (* Parameter next_provenance_neq : *)
+  (*   forall pr, *)
+  (*     pr <> next_provenance pr. *)
+
+  (* Debug *)
+  Parameter show_prov : Prov -> string.
+  Parameter show_provenance : Provenance -> string.
+  Parameter show_allocation_id : AllocationId -> string.
+
+  (* (* Hints *) *)
+  (* Hint Resolve *)
+  (*      provenance_lt_trans *)
+  (*      provenance_lt_next_provenance *)
+  (*      provenance_lt_nrefl : PROVENANCE_LT. *)
+  
+End PROVENANCE.
+
+
+(* (* Derived functions on provenances. *) *)
+(* Module PROV_FUNCS(Addr : ADDRESS) (PROV : PROVENANCE(Addr)). *)
+(*   Import PROV. *)
+
+(*   Definition all_accesses_allowed (pr : Prov) (aids : list AllocationId) : bool *)
+(*     := forallb (access_allowed pr) aids. *)
+
+(*   Definition all_aid_accesses_allowed (pr : AllocationId) (aids : list AllocationId) : bool *)
+(*     := forallb (aid_access_allowed pr) aids. *)
+
+(*   Lemma allocation_id_to_prov_provenance_to_allocation_id_inv : *)
+(*     forall pr pr', *)
+(*       allocation_id_to_prov (provenance_to_allocation_id pr) = allocation_id_to_prov (provenance_to_allocation_id pr') -> *)
+(*       pr = pr'. *)
+(*   Proof. *)
+(*     intros pr pr' H. *)
+(*     apply provenance_to_allocation_id_inv. *)
+(*     apply allocation_id_to_prov_inv. *)
+(*     auto. *)
+(*   Qed. *)
+(* End PROV_FUNCS. *)
+
