src/rocq/Semantics/Params/VellvmImplem/Address.v
@@ -1,0 +1,38 @@
+From Vellvm Require Import
+  Utilities
+  Syntax.
+
+From Vellvm Require Import
+  Rocqlib
+  Params.IPtr
+  Params.Address
+  VellvmImplem.Provenance
+  VellvmIntegers.
+
+From QuickChick Require Import Show.
+
+Module Address (IP : IPTR) <: ADDRESS Provenance.
+
+  Module P := Provenance.
+  Import IP P.
+
+  Definition addr := (intptr * Prov) % type.
+  Definition null : addr := (zero, nil_prov)%Z.
+
+  (* TODO: is this what we should be using for equality on pointers? Probably *NOT* because of provenance. *)
+  Lemma eq_dec : forall (a b : addr), {a = b} + {a <> b}.
+  Proof.
+    intros [a1 a2] [b1 b2].
+    destruct (IP.eq_dec a1 b1); destruct (option_eq (list_eq_dec P.eq_dec) a2 b2); subst.
+    - left; reflexivity.
+    - right. intros H. inversion H; subst. apply n. reflexivity.
+    - right. intros H. inversion H; subst. apply n. reflexivity.
+    - right. intros H. inversion H; subst. apply n. reflexivity.
+  Qed.
+
+  Definition show_addr (a : addr) :=
+    match a with
+    | (i, p) => show (show_intptr i, show_prov p)
+    end.
+  
+End Address.
