src/rocq/Semantics/Params/VellvmImplem/IPtrFinite.v
@@ -1,0 +1,208 @@
+(* Used in [to_Z_inj] *)
+From Stdlib Require Import ProofIrrelevance.
+
+From Vellvm Require Import
+  Utilities
+  Syntax.
+
+From Vellvm Require Import
+  IPtr
+  Integers
+  VellvmIntegers.
+
+From QuickChick Require Import Show.
+
+Module IP64Bit : IPTR.
+(*   with *)
+(* Definition intptr := int64 with *)
+(* Definition zero := (@Integers.zero 64) with *)
+(* Definition from_Z := @from_Z_bits 64 with *)
+(* Definition to_Z := @Integers.unsigned 64 with *)
+(* Definition VMemInt_intptr := @VMemInt_intptr_ix 64. *)
+
+  Definition from_Z_bits {sz : positive} : Z -> EOB (@bit_int sz) :=
+    (fun (x : Z) =>
+       if (x <=? @Integers.max_unsigned sz)%Z && (x >=? 0)%Z
+       then ret (@Integers.repr sz x)
+       else raise_oom "IPBit from_Z oom.").
+
+  Instance VMemInt_intptr_ix {sz : positive} : VMemInt (@bit_int sz)
+    :=
+    { (* Comparisons *)
+      mequ := @Integers.eq sz;
+      mcmp := @Integers.cmp sz;
+      mcmpu := @Integers.cmpu sz;
+      msamesign := fun _ _ => true;
+      
+      (* Constants *)
+      mbitwidth := Some sz;
+      mzero := @Integers.zero sz;
+      mone := @Integers.one sz;
+
+      (* Arithmetic *)
+      madd := fun x y =>
+                if (Integers.eq (Integers.add_carry x y (@Integers.zero sz)) (@Integers.one sz))
+                then raise_oom "IPBit addition overflow."
+                else ret (Integers.add x y);
+      madd_carry := fun x y c => (@Integers.zero sz);
+      madd_overflow := fun x y c => (@Integers.zero sz);
+
+      msub := fun x y =>
+                if (@Integers.unsigned sz y >? @Integers.unsigned sz x)%Z
+                then raise_oom "IPBit subtraction underflow."
+                else ret (@Integers.sub sz x y);
+      msub_borrow := fun x y c => (@Integers.zero sz);
+      msub_overflow := fun x y c => (@Integers.zero sz);
+
+      mmul :=
+        fun x y =>
+          let res := ((Integers.unsigned x) * (Integers.unsigned y))%Z in
+          if (res >? @Integers.max_unsigned 64)
+          then raise_oom "IPBit multiplication overflow."
+          else ret (@Integers.repr sz res);
+
+      mdivu := @Integers.divu sz;
+      mdivs := fun _ _ => raise_oom "IPBit signed division.";
+
+      mmodu := @Integers.modu sz;
+      mmods := fun _ _ => raise_oom "IPBit signed modulo.";
+
+      mshl :=
+        fun x y =>
+          let res_Z := Z.shiftl (@Integers.unsigned sz x) (@Integers.unsigned sz y) in
+          if res_Z >? @Integers.max_unsigned sz
+          then raise_oom "IP64Bit left shift overflow."
+          else ret (@Integers.repr sz res_Z);
+      mshr := @Integers.shr sz;
+      mshru := @Integers.shru sz;
+
+      mnegative := fun _ => raise_oom "IP64Bit taking negative of a number.";
+
+      (* Logic *)
+      mand := @Integers.and sz;
+      mor := @Integers.or sz;
+      mxor := @Integers.xor sz;
+
+      (* Bounds *)
+      mmin_signed := ret (@Integers.min_signed sz);
+      mmax_signed := ret (@Integers.max_signed sz);
+      mmax_unsigned := ret (@Integers.max_unsigned sz);
+
+      (* Conversion *)
+      munsigned := @Integers.unsigned sz;
+      msigned := @Integers.signed sz;
+
+      mrepr := @from_Z_bits sz;
+
+      mdtyp_of_int := DTYPE_IPTR
+    }.
+
+  Definition intptr := int64.
+  Definition zero := (@Integers.zero 64).
+
+  Definition eq_dec := @Integers.eq_dec 64.
+  Definition eqb := @Integers.eq 64.
+
+  Definition to_Z (x : intptr) := Integers.unsigned x.
+
+  Definition VMemInt_intptr := @VMemInt_intptr_ix 64.
+
+  (* TODO: negatives.... ???? *)
+  Definition to_unsigned := to_Z.
+  Definition from_Z (x : Z) : EOB intptr := @from_Z_bits 64 x.
+
+  Definition show_intptr (p : intptr) : string := show (unsigned p).
+    
+  Lemma from_Z_to_Z :
+    forall (z : Z) (i : intptr),
+      from_Z z = ret i ->
+      to_Z i = z.
+  Proof.
+    intros z i FROM.
+    unfold from_Z, from_Z_bits in FROM.
+    break_match_hyp; inversion FROM.
+    unfold to_Z.
+    apply Integers.unsigned_repr.
+    lia.
+  Qed.
+
+  Lemma from_Z_injective :
+    forall (z1 z2 : Z) (i : intptr),
+      from_Z z1 = ret i ->
+      from_Z z2 = ret i ->
+      z1 = z2.
+  Proof.
+    intros z1 z2 i Z1 Z2.
+    unfold from_Z, from_Z_bits in *.
+    break_match_hyp; inversion Z2.
+    break_match_hyp; inversion Z1.
+    pose proof (@Integers.unsigned_repr 64 z1).
+    pose proof (@Integers.unsigned_repr 64 z2).
+    forward H; try lia.
+    forward H2; try lia.
+    congruence.
+  Qed.
+
+  Lemma to_Z_from_Z :
+    forall (i : intptr),
+      from_Z (to_Z i) = ret i.
+  Proof.
+    intros i.
+    unfold from_Z, from_Z_bits, to_Z.
+    break_match.
+    - rewrite Integers.repr_unsigned; auto.
+    - unfold intptr in *.
+      pose proof Integers.unsigned_range i.
+      unfold Integers.max_unsigned in *.
+      lia.
+  Qed.
+
+  Lemma from_Z_0 :
+    from_Z 0 = ret zero.
+  Proof.
+    auto.
+  Qed.
+
+  Lemma to_Z_0 :
+    to_Z zero = 0%Z.
+  Proof.
+    auto.
+  Qed.
+
+  (* TODO : do we need this? Should we assume and leverage it more broadly? *)
+  Lemma to_Z_inj :
+    forall x y,
+      to_Z x = to_Z y ->
+      x = y.
+  Proof.
+    intros x y EQ.
+    unfold to_Z in *.
+    destruct x, y.
+    unfold Integers.unsigned in *.
+    cbn in *; subst.
+    rewrite (proof_irrelevance _ intrange intrange0); auto.
+  Qed.
+
+  Lemma VMemInt_intptr_dtyp :
+    @mdtyp_of_int intptr VMemInt_intptr = DTYPE_IPTR.
+  Proof.
+    cbn. reflexivity.
+  Qed.
+
+  Lemma VMemInt_intptr_mrepr_from_Z :
+    forall x,
+      @mrepr intptr VMemInt_intptr x = from_Z x.
+  Proof.
+    reflexivity.
+  Qed.
+
+  Lemma to_Z_to_unsigned :
+    forall x,
+      to_Z x = to_unsigned x.
+  Proof.
+    intros x.
+    reflexivity.
+  Qed.
+
+End IP64Bit.
+
