src/rocq/Semantics/Params/VellvmImplem/Provenance.v
@@ -1,0 +1,74 @@
+From Vellvm Require Import
+  Utilities
+  Syntax.
+
+From Vellvm Require Import
+  Params.IPtr
+  Params.Provenance
+  Integers
+  VellvmIntegers.
+
+From QuickChick Require Import Show.
+
+Module Provenance <: PROVENANCE.
+
+  Definition Provenance := N.
+  Definition AllocationId := option Provenance. (* None is wildcard *)
+  (* TODO: Should probably make this an NSet, but it gives universe inconsistency with Module addr *)
+  Definition Prov := option (list Provenance). (* Provenance *)
+
+  Definition wildcard_prov : Prov := None.
+  Definition nil_prov : Prov := Some [].
+
+  (* Does the provenance set pr allow for access to aid? *)
+  Definition access_allowed (pr : Prov) (aid : AllocationId) : bool
+    := match pr with
+       | None => true (* Wildcard can access anything. *)
+       | Some prset =>
+         match aid with
+         | None => true (* Wildcard, can be accessed by anything. *)
+         | Some aid =>
+           existsb (N.eqb aid) prset
+         end
+       end.
+
+  Definition aid_access_allowed (pr : AllocationId) (aid : AllocationId) : bool
+    := match pr with
+       | None => true
+       | Some pr =>
+         match aid with
+         | None => true
+         | Some aid =>
+           N.eqb pr aid
+         end
+       end.
+
+  Definition allocation_id_to_prov (aid : AllocationId) : Prov
+    := fmap (fun x => [x]) aid.
+
+  Definition provenance_to_allocation_id (pr : Provenance) : AllocationId
+    := Some pr.
+
+  Definition provenance_to_prov (pr : Provenance) : Prov
+    := Some [pr].
+
+  Definition next_provenance (pr : Provenance) : Provenance
+    := N.succ pr.
+
+  Definition initial_provenance : Provenance
+    := 0%N.
+
+  Lemma eq_dec :
+    forall (pr pr' : Provenance),
+      {pr = pr'} + {pr <> pr'}.
+  Proof.
+    exact N.eq_dec.
+  Defined.
+
+    (* Debug *)
+  Definition show_prov (pr : Prov) := Show.show pr.
+  Definition show_provenance (pr : Provenance) := Show.show pr.
+  Definition show_allocation_id (aid : AllocationId) := Show.show aid.
+
+End Provenance.
+
